WIP

theories/prob_eff_lang/probblaze/examples/DH_KE/new_schan_ri.v
@@ -307,7 +307,9 @@ Section schan_security.
 (*Verification of F_OAUTH[F_KE_L[CHAN[]]] ≤ CHAN_SIM[F_CHAN[]]*)
 (*----------------------------------------------------------*)
 Lemma F_KE_CHAN_SIM (f1 f2 : val) (L : sem_row Σ) :
-    sem_val_typed f1 f2 ((∀ᵣ θₕ, (((⊤ × (sem_ty_sum 𝟙 𝟙)) -{ θₕ }-> (Option  ⊤)) × ((sem_ty_sum 𝟙 𝟙) -{ θₕ }-> (Option  ⊤))) -{ sem_row_union  θₕ L }-> 𝟙))%T -∗ 
+  (* sem_val_typed f1 f2 ((∀ᵣ θₕ, (((⊤ × (sem_ty_sum 𝟙 𝟙)) -{ θₕ }-> (Option  ⊤)) × ((sem_ty_sum 𝟙 𝟙) -{ θₕ }-> (Option  ⊤))) -{ sem_row_union  θₕ L }-∘ 𝟙))%T -∗*)
+   (∀ᵣ θₕ, (((⊤ × 𝟙 + 𝟙) -{ θₕ }-> Option ⊤) × 𝟙 + 𝟙 -{ θₕ }-> Option ⊤) -{ sem_row_union θₕ L }-∘ 𝟙)%T
+                 f1 f2 -∗
     BREL REAL_CHAN f1
       ≤ CHAN_SIM (F_CHAN f2) <|⊥|> {{λ v1 v2,
                                        ∀ (leakauth1 leakauth2 keyleak1 keyleak2 : label),
@@ -433,13 +435,13 @@ Proof with (repeat foldkont) using G H cg inG0 inG1 inG2 klk1 klk2 lka1 lka2 vg 
          end
                  end )%E).
   
-  unfold sem_val_typed. simpl.
-  iDestruct "Hrelf1f2" as "#Hrelf1f2".
+  (*unfold sem_val_typed. simpl.
+  iDestruct "Hrelf1f2" as "#Hrelf1f2".*)
   set (θ := client_row channel' leaksec' getKey' schannel_l schannel_r).
   iSpecialize ("Hrelf1f2" $! θ).
-  iDestruct "Hrelf1f2" as "#Hrelf1f2".
+  (*iDestruct "Hrelf1f2" as "#Hrelf1f2".*)
   unfold sem_ty_arr, sem_ty_mbang. simpl.
-  iDestruct "Hrelf1f2" as "#Hrelf1f2". 
+  (*iDestruct "Hrelf1f2" as "#Hrelf1f2".*)
   iAssert (sem_val_typed  ((λ: "m", do: schannel_l InjL "m"), (λ: "m", do: schannel_l InjR "m"))%V ((λ: "m", do: schannel_r InjL "m") , (λ: "m", do: schannel_r InjR "m"))%V (((⊤ ×(𝟙 + 𝟙))%T -{ θ }-> (Option ⊤)) × ((𝟙 + 𝟙)%T -{ θ }-> (Option ⊤)))%T) as "Hschn".
   { iApply SEM_TYPED_EFF. }
   (*iAssert (sem_val_typed (λ: "m", do: schannel_l InjR "m") (λ: "m", do: schannel_r InjR "m") ((𝟙 + 𝟙)%T -{ θ }-> (Option 𝔾))%T) as "Hschnrcv".
@@ -923,7 +925,9 @@ Print sem_val_typed.
  *)
 
 Lemma SEM_F_KE_CHAN_SIM (f1 f2 : val) (L : sem_row Σ) :
-    sem_val_typed f1 f2 ((∀ᵣ θₕ, (((⊤ × (sem_ty_sum 𝟙 𝟙)) -{ θₕ }-> (Option ⊤)) × ((sem_ty_sum 𝟙 𝟙) -{ θₕ }-> (Option ⊤))) -{ sem_row_union  θₕ L }-> 𝟙))%T -∗ 
+  (* sem_val_typed f1 f2 ((∀ᵣ θₕ, (((⊤ × (sem_ty_sum 𝟙 𝟙)) -{ θₕ }-> (Option ⊤)) × ((sem_ty_sum 𝟙 𝟙) -{ θₕ }-> (Option ⊤))) -{ sem_row_union  θₕ L }-∘ 𝟙))%T -∗*)
+   (∀ᵣ θₕ, (((⊤ × 𝟙 + 𝟙) -{ θₕ }-> Option ⊤) × 𝟙 + 𝟙 -{ θₕ }-> Option ⊤) -{ sem_row_union θₕ L }-∘ 𝟙)%T
+                 f1 f2 -∗
     BREL REAL_CHAN f1
       ≤ CHAN_SIM (F_CHAN f2) <|⊥|> {{λ v1 v2,
                                        (* (∀ᵣ θ₁,  (((⊤ × (𝟙 + 𝟙)) -{ θ₁ }-> 𝟙) × ((𝟙 + 𝟙) -{ θ₁ }-> Option ⊤)) ⊸ ((𝟙 + 𝟙) -{ θ₁ }-> Option ⊤) -{ sem_row_union θ₁ L }-∘ 𝟙)%T v1 v2 }}.*)
@@ -933,17 +937,25 @@ Admitted.
  
 Lemma REAL_CHAN_CHAN_SIM_F_CHAN :
   ⊢ sem_val_typed (REAL_CHAN)%V (λ: "f", CHAN_SIM (F_CHAN "f"))%V
-      (∀ᵣ θ__L ,(∀ᵣ θₕ, (((⊤ × (sem_ty_sum 𝟙 𝟙)) -{ θₕ }-> (Option ⊤)) × ((sem_ty_sum 𝟙 𝟙) -{ θₕ }-> (Option  ⊤))) -{ sem_row_union  θₕ θ__L }-> 𝟙) ⊸ (*type of client*)
+      (∀ᵣ θ__L ,(∀ᵣ θₕ, (((⊤ × (sem_ty_sum 𝟙 𝟙)) -{ θₕ }-> (Option ⊤)) × ((sem_ty_sum 𝟙 𝟙) -{ θₕ }-> (Option  ⊤))) -{ sem_row_union  θₕ θ__L }-∘ 𝟙) ⊸ (*type of client*)
                (* (∀ᵣ θ₁,  (((⊤ × (𝟙 + 𝟙)) -{ θ₁ }-> 𝟙) × ((𝟙 + 𝟙) -{ θ₁ }-> Option ⊤)) ⊸ ((𝟙 + 𝟙) -{ θ₁ }-> Option ⊤) -{ sem_row_union θ₁ θ__L }-∘ 𝟙))%T.*) 
       (∀ᵣ θ₁, ∀ᵣ θ₂,  (((⊤ × (𝟙 + 𝟙)) -{ θ₁ }-> 𝟙) × ((𝟙 + 𝟙) -{ θ₁ }-> Option ⊤)) ⊸ ((𝟙 + 𝟙) -{ θ₂ }-> Option ⊤) -{ sem_row_union (sem_row_union θ₁ θ₂) θ__L }-∘ 𝟙))%T.
 Proof using G inG0 inG1 inG2.   
   iModIntro. iIntros (L).
-  iIntros (f1 f2) "#Hrelf1f2".
+  iIntros (f1 f2) "Hrelf1f2".
   brel_pures'.
+  simpl.
+  assert (to_iThyIfMono OS [] = []) as <- by done.
+  iApply (brel_mono OS with "[][Hrelf1f2]");
+  [iApply to_iThy_le_refl|simpl|simpl].
   About brel_wand.
-  iApply brel_wand.
-  + iApply (SEM_F_KE_CHAN_SIM _ _ L). by iModIntro.
-  + iIntros (??). iModIntro. iIntros "H". iApply "H".
+  About brel_mono.
+  About brel_wand.
+(*  iApply (brel_mono with " [Hrelf1f2][]").
+  iApply (brel_wand with "Hrelf1f2").*)
+  +  iApply (SEM_F_KE_CHAN_SIM _ _ L).
+     iApply "Hrelf1f2".
+  + iIntros (??) "$". 
 Qed.
      (* (∀ᵣ θ__L, (∀ᵣ θₕ,(((sem_ty_sum 𝟙 𝟙) -{ θₕ }-> (Option  𝔾)) × ((sem_ty_sum 𝟙 𝟙) -{ θₕ }-> (Option  𝔾))) - {sem_row_union θₕ θ__L} -> 𝟙)%T   (*type of the client *)
            ⊸  (∀ᵣ θₗ,  (((⊤ × (𝟙 + 𝟙)) -{ θₗ }-> 𝟙) × ((𝟙 + 𝟙) -{ θₗ }-> Option ⊤)) ⊸ ((𝟙 + 𝟙) -{ θₗ }-> Option ⊤)   (*thunks for effect operations being passed as arguments *)
@@ -956,7 +968,7 @@ Print sem_typed.*)
 (*----------------------------------------------------------------*)
 Lemma REAL_IDEAL_SCHAN :
   ⊢ sem_typed [] REAL_CHAN (λ: "f", (CHAN_SIM (F_CHAN "f")))%V ⊥
-       (∀ᵣ θ__L ,(∀ᵣ θₕ, (((⊤ × (sem_ty_sum 𝟙 𝟙)) -{ θₕ }-> (Option ⊤)) × ((sem_ty_sum 𝟙 𝟙) -{ θₕ }-> (Option  ⊤))) -{ sem_row_union  θₕ θ__L }-> 𝟙)%T ⊸ (*type of client*)
+       (∀ᵣ θ__L ,(∀ᵣ θₕ, (((⊤ × (sem_ty_sum 𝟙 𝟙)) -{ θₕ }-> (Option ⊤)) × ((sem_ty_sum 𝟙 𝟙) -{ θₕ }-> (Option  ⊤))) -{ sem_row_union  θₕ θ__L }-∘ 𝟙)%T ⊸ (*type of client*)
                  (* (∀ᵣ θ₁,  (((⊤ × (𝟙 + 𝟙)) -{ θ₁ }-> 𝟙) × ((𝟙 + 𝟙) -{ θ₁ }-> Option ⊤)) ⊸ ((𝟙 + 𝟙) -{ θ₁ }-> Option ⊤) -{ sem_row_union θ₁ θ__L }-∘ 𝟙))%T [].*)
                  (∀ᵣ θ₁, ∀ᵣ θ₂,  (((⊤ × (𝟙 + 𝟙)) -{ θ₁ }-> 𝟙) × ((𝟙 + 𝟙) -{ θ₁ }-> Option ⊤)) ⊸ ((𝟙 + 𝟙) -{ θ₂ }-> Option ⊤) -{ sem_row_union (sem_row_union θ₁ θ₂) θ__L }-∘ 𝟙))%T [].
 Proof using G inG0 inG1 inG2 klk1 klk2 lka1 lka2. 
@@ -976,7 +988,649 @@ Qed.
  
 (*Lemma IDEAl_REAL_SCHAN :*)
 
+Definition R_CHAN : val :=
+   λ: "f",
+      (F_KE_L ||ᵣ F_OAUTH) (CHAN "f").
 
-
+(*Verification of F_KE_L[F_OAUTH[CHAN[]]] ≤ CHAN_SIM[F_CHAN[]]*)
+(*----------------------------------------------------------*)
+Lemma F_OAUTH_CHAN_SIM (f1 f2 : val) (L : sem_row Σ) :
+  (* sem_val_typed f1 f2 ((∀ᵣ θₕ, (((⊤ × (sem_ty_sum 𝟙 𝟙)) -{ θₕ }-> (Option  ⊤)) × ((sem_ty_sum 𝟙 𝟙) -{ θₕ }-> (Option  ⊤))) -{ sem_row_union  θₕ L }-∘ 𝟙))%T -∗*)
+   (∀ᵣ θₕ, (((⊤ × 𝟙 + 𝟙) -{ θₕ }-> Option ⊤) × 𝟙 + 𝟙 -{ θₕ }-> Option ⊤) -{ sem_row_union θₕ L }-∘ 𝟙)%T
+                 f1 f2 -∗
+    BREL R_CHAN f1
+      ≤ CHAN_SIM (F_CHAN f2) <|⊥|> {{λ v1 v2,
+                                       ∀ (leakauth1 leakauth2 keyleak1 keyleak2 : label),
+                                       BREL v1 (λ: "m", do: keyleak1 "m")%V ((λ: "m", do: leakauth1 (Send "m")), (λ: "m", do: leakauth1 (Recv "m")))%V ≤ v2 ((λ: "m", do: leakauth2 (Send "m")), (λ: "m", do: leakauth2 (Recv "m")))%V  (λ: "m", do: keyleak2 "m")%V  <| (iLblSig_to_iLblThy (envsec_row keyleak1 keyleak2 leakauth1 leakauth2 )) ++ (iLblSig_to_iLblThy L) |> {{ (λ w1 w2, 𝟙%T w1 w2)}}}}.
+Proof with (repeat foldkont) using G H cg inG0 inG1 inG2 klk1 klk2 lka1 lka2 vg vgg Σ.
+  iIntros "Hrelf1f2".
+  repeat simpl.
+  unfold R_CHAN. brel_pures.
+  unfold right_composition. brel_pures.
+  unfold CHAN.
+  repeat simpl. brel_pures'.
+  
+  (*unfold CHAN_SIM, F_OAUTH.*)
+  unfold F_CHAN, CHAN_SIM, F_KE_L, F_OAUTH. 
+   
+  repeat simpl. brel_pures. iModIntro. iIntros (????).
+  brel_pures.
+  iApply brel_alloctape_r. iIntros (α) "Hα". brel_pures_r. 
+  iApply brel_alloc_r. iIntros (l_sim) "Hl_sim". brel_pures_r.
+  iApply brel_couple_UT. 1: auto.
+  simpl. iFrame "Hα". iSplit => //.
+  iIntros (n ?) "!> Hα". brel_pures.
+  brel_exp_l. brel_pures. 
+  iApply brel_effect_r. iIntros (leaksec') "Hleaksec !>". brel_pures.
+  iApply brel_alloc_r. iIntros (l_fchan) "Hlfchan". brel_pures_r.
+  iApply brel_effect_l. iIntros (getKey') "!> HgK !>". brel_pures_l.
+  iApply brel_alloc_l. iIntros (l_rchan) "!>Hlrchan". brel_pures_l.
+  iApply brel_effect_l. iIntros (channel') "!> Hchannel !>". brel_pures_l.
+  iApply brel_effect_r. iIntros (schannel_r) "Hschannel_r !>". brel_pures_r.
+  iApply brel_alloc_l. iIntros (l_auth) "!>Hl_auth". brel_pures_l.
+  iApply brel_effect_l. iIntros (schannel_l) "!> Hschannel_l !>". brel_pures_l.
+ (* iApply brel_alloc_r. iIntros (l_fchan) "Hlfchan". brel_pures_r.
+  iApply brel_effect_r. iIntros (schannel_r) "Hschannel_r !>". brel_pures_r.
+  iApply brel_couple_UT. 1: auto.
+  simpl. iFrame "Hα". iSplit => //.
+  iIntros (n ?) "!> Hα". brel_pures.
+  brel_exp_l. brel_pures.
+  iApply brel_effect_l. iIntros (getKey') "!> HgK !>". brel_pures_l.
+  iApply brel_effect_r. iIntros (leaksec') "Hleaksec !>". brel_pures.
+  iApply brel_alloc_r. iIntros (l_fchan) "Hlfchan". brel_pures_r.
+  iApply brel_effect_r. iIntros (schannel_r) "Hschannel_r !>". brel_pures_r.
+  brel_pures'. repeat simpl. brel_pures'.
+  iApply brel_alloc_l. iIntros (l_auth) "!>Hl_auth". brel_pures_l.
+  iApply brel_effect_l. iIntros (channel') "!> Hchannel !>". brel_pures_l.
+  iApply brel_couple_UT. 1: auto.
+  simpl. iFrame "Hα". iSplit => //.
+  iIntros (n ?) "!> Hα". brel_pures.
+  brel_exp_l. brel_pures.
+  iApply brel_effect_l. iIntros (getKey') "!> HgK !>". brel_pures_l.
+  iApply brel_effect_r. iIntros (leaksec') "Hleaksec !>". brel_pures.
+  iApply brel_alloc_r. iIntros (l_fchan) "Hlfchan". brel_pures_r.
+  iApply brel_effect_r. iIntros (schannel_r) "Hschannel_r !>". brel_pures_r.
+  brel_pures'. repeat simpl. brel_pures'.
+  iApply brel_alloc_l. iIntros (l_rchan) "!>Hlrchan". brel_pures_l.
+  iApply brel_effect_l. iIntros (schannel_l) "!> Hschannel_l !>". brel_pures_l. *)
+  set (kl1 := ( match: "payload" with
+         InjL "payload" =>
+           let: "dst" := "payload" in
+           let: "m" := Fst "dst" in
+           let: "dst" := Snd "dst" in
+           match: ! #l_auth with
+             InjL <> =>
+               #l_auth <- InjR "m";; 
+               let: "key" := (λ: "party", do: getKey' "party")%V "dst" in
+               match: "key" with
+                 InjL <> => "k" #()%V
+               | InjR "x" =>
+                 let: "enc_m" := xor "x" "m" in
+                 (λ: "m", do: channel' InjL "m")%V ("enc_m", bob);; "k" #()%V
+               end
+           | InjR "m" => "k" #()%V
+           end
+       | InjR "from" =>
+         let: "key" := (λ: "party", do: getKey' "party")%V "from" in
+         match: "key" with
+           InjL <> => "k" (InjLV #()%V)
+         | InjR "key" =>
+           let: "r" := (λ: "m", do: channel' InjR "m")%V "from" in
+           match: "r" with
+             InjL <> => "k" (InjLV #()%V)
+           | InjR "x" => let: "enc_m" := xor "key" "x" in "k" (InjR "enc_m")
+           end
+         end
+       end)%E).
+  set (kl2 := ( match: "payload" with
+         InjL "payload" =>
+           let: "dst" := "payload" in
+           let: "m" := Fst "dst" in
+           let: "dst" := Snd "dst" in
+           match: ! #l_rchan with
+             InjL <> =>
+               #l_rchan <- InjR "m";; 
+               (λ: "m", do: leakauth1 Send "m")%V ("m", "dst");; "k" #()%V
+           | InjR "message" => "k" #()%V
+           end
+       | InjR "from" =>
+         let: "r" := (λ: "m", do: leakauth1 Recv "m")%V "from" in
+         match: "r" with InjL <> => "k" (InjLV #()%V) | InjR "x" => "k" ! #l_rchan end
+       end)%E).
+  set (kl3 := ( match: "p" with
+         InjL <> =>
+           (λ: "m", do: keyleak1 "m")%V (InjL bob);; 
+           let: "r" := (λ: "m", do: keyleak1 "m")%V (InjR bob) in
+           match: "r" with
+             InjL <> => "k" (InjLV #()%V)
+           | InjR "w" => "k" (InjR (vgval (g ^+ n)))
+           end
+       | InjR <> =>
+         let: "r" := (λ: "m", do: keyleak1 "m")%V (InjR alice) in
+         match: "r" with
+           InjL <> => "k" (InjLV #()%V)
+         | InjR "w" =>
+           (λ: "m", do: keyleak1 "m")%V (InjL alice);; "k" (InjR (vgval (g ^+ n)))
+         end
+       end)%E).
+  set (kr1 := (  match: "payload" with
+         InjL "payload" =>
+           let: "dst" := "payload" in
+           let: "m" := Fst "dst" in
+           let: "dst" := Snd "dst" in
+           match: ! #l_fchan with
+             InjL <> => #l_fchan <- InjR "m";; (λ: "m", do: leaksec' InjL "m")%V "dst";; "k" #()%V
+           | InjR "x" => "k" #()%V
+           end
+       | InjR "from" =>
+         let: "r" := (λ: "m", do: leaksec' InjR "m")%V "from" in
+         match: "r" with InjL <> => "k" (InjLV #()%V) | InjR "x" => "k" (InjR "x") end
+                 end)%E).
+  set (kr2 := (  match: "payload" with
+         InjL "payload" =>
+           (λ: "m", do: keyleak2 "m")%V (InjL bob);; 
+           let: "r" := (λ: "m", do: keyleak2 "m")%V (InjR bob) in
+           match: "r" with
+             InjL <> => "k" (InjLV #()%V)
+           | InjR "x" =>
+             match: ! #l_sim with
+               InjL <> =>
+                 let: "m'" := #()%V;; rand(#lbl:α) #(S n'') in
+                 let: "mA" := vexp g "m'" in
+                 #l_sim <- InjR "m'";; (λ: "m", do: leakauth2 Send "m")%V ("mA", bob);; "k" #()%V
+             | InjR "m" => "k" #()%V
+             end
+           end
+       | InjR "from" =>
+         (λ: "m", do: keyleak2 "m")%V (InjL "from");; 
+         let: "r" := (λ: "m", do: keyleak2 "m")%V (InjR "from") in
+         match: "r" with
+           InjL <> => "k" (InjLV #()%V)
+         | InjR "x" =>
+           let: "rla" := (λ: "m", do: leakauth2 Recv "m")%V "from" in
+           match: "rla" with InjL <> => "k" (InjLV #()%V) | InjR "x" => "k" ! #l_sim end
+         end
+                 end )%E).
+  
+  (*unfold sem_val_typed. simpl.
+  iDestruct "Hrelf1f2" as "#Hrelf1f2".*)
+  set (θ := client_row channel' leaksec' getKey' schannel_l schannel_r).
+  iSpecialize ("Hrelf1f2" $! θ).
+  (*iDestruct "Hrelf1f2" as "#Hrelf1f2".*)
+  unfold sem_ty_arr, sem_ty_mbang. simpl.
+  (*iDestruct "Hrelf1f2" as "#Hrelf1f2".*)
+  iAssert (sem_val_typed  ((λ: "m", do: schannel_l InjL "m"), (λ: "m", do: schannel_l InjR "m"))%V ((λ: "m", do: schannel_r InjL "m") , (λ: "m", do: schannel_r InjR "m"))%V (((⊤ ×(𝟙 + 𝟙))%T -{ θ }-> (Option ⊤)) × ((𝟙 + 𝟙)%T -{ θ }-> (Option ⊤)))%T) as "Hschn".
+  { iApply SEM_TYPED_EFF. }
+  (*iAssert (sem_val_typed (λ: "m", do: schannel_l InjR "m") (λ: "m", do: schannel_r InjR "m") ((𝟙 + 𝟙)%T -{ θ }-> (Option 𝔾))%T) as "Hschnrcv".
+  { admit. }*)
+  unfold sem_val_typed. simpl.
+  iDestruct "Hschn" as "#Hschn".
+  (*iDestruct "Hschnrcv" as "#Hschnrcv".*)
+  iSpecialize ("Hrelf1f2" with "Hschn"). simpl.
+  (*About brel_add_label_l.*)
+  (*iSpecialize ("Hrelf1f2" with "Hschnrcv").
+  brel_pures'.*)
+ 
+  (*iAssert (brel ⊤ (f1 ((λ: "m", do: schannel_l InjL "m"),(λ: "m", do: schannel_l InjR "m"))%V)
+              (f2 ((λ: "m", do: schannel_r InjL "m"),(λ: "m", do: schannel_r InjR "m"))%V)
+    (([channel; getKey1; schannel1], [leaksec; schannel2], sec_channel schannel1 schannel2)
+      :: iLblSig_to_iLblThy L) 𝟙%T) as "Hrelf1f2mono".
+  { admit. }*)
+   iApply (brel_na_alloc
+              (((α ↪ₛN (S n''; [n])) ∗ l_sim ↦ₛ NONEV ∗ l_auth ↦ NONEV)
+               ∨ (α ↪ₛ□ (S n''; []) ∗ l_sim ↦ₛ□ SOMEV #n ∗  l_auth ↦□ SOMEV (xor (vgval $ g ^+n)%g #0)))%I
+              alphaN).
+   iSplitL "Hα Hl_sim Hl_auth"; [iNext; iFrame; iLeft; iFrame|].
+   iIntros "#Hinvα".
+   iApply (brel_na_alloc
+              ((l_fchan ↦ₛ NONEV ∗ l_rchan ↦ NONEV)
+               ∨ (l_fchan ↦ₛ□ SOMEV #0 ∗  l_rchan ↦□ SOMEV #0))%I
+              betaN).
+   iSplitL  "Hlrchan Hlfchan"; [iNext; iFrame; iLeft; iFrame|].
+   iIntros "#Hinvβ" .
+   (*set (f'1 := ( handle: f1 (λ: "m", do: schannel_l InjL "m", λ: "m", do: schannel_l InjR "m")%V with
+     | effect schannel_l "payload", rec "k" as multi => kl1
+               | return "y" => #()%V end)%E).
+   set (f'2 := ( handle: f2 (λ: "m", do: schannel_r InjL "m", λ: "m", do: schannel_r InjR "m")%V with
+     | effect schannel_r "payload", rec "k" as multi => kr1
+     | return "y" => #()%V
+                 end)%E).
+   iApply brel_new_theory.
+   iApply (brel_add_label_l with "HgK").
+   iApply (brel_add_label_l with "Hchannel").
+   iApply (brel_add_label_r with "Hleaksec").
+   
+   iApply ((brel_exhaustion f'1 f'2 _ _ _ _ _ _ _ _ _ )); try simpl.
+   { admit.}
+   { admit.}
+   { 
+   About brel_exhaustion.
+   unfold f'1, f'2.*) 
+   iApply brel_new_theory.
+   iApply (brel_add_label_l with "Hschannel_l").
+   iApply (brel_add_label_r with "Hschannel_r").
+   iApply (brel_add_label_l with "HgK").
+   iApply (brel_add_label_l with "Hchannel").
+   iApply (brel_add_label_r with "Hleaksec").
+   set (X :=  iLblSig_to_iLblThy [([schannel_l] , [schannel_r] , sec_channel schannel_l schannel_r)]).
+   set (R := (λ u1 u2 : val, 𝟙%T u1 u2)).
+   set (X' := sec_channel schannel_l schannel_r).
+   (*iAssert  (brel ⊤ (f1 (λ: "m", do: schannel_l InjL "m", λ: "m", do: schannel_l InjR "m")%V)
+    (f2 (λ: "m", do: schannel_r InjL "m", λ: "m", do: schannel_r InjR "m")%V)
+    (([channel'; getKey'; schannel_l], [leaksec'; schannel_r], X)
+     :: ([keyleak1], [keyleak2], keyleak keyleak1 keyleak2)
+        :: ([leakauth1], [leakauth2], leakauth leakauth1 leakauth2) :: iLblSig_to_iLblThy L)
+    R) as "Hrelf1f2mono".*)
+   About brel_exhaustion.
+   Print distinct'.
+   Print distinct_l.
+   iApply brel_learn. iIntros "%Hdist' _". 
+   iApply ((brel_exhaustion (f1 ((λ: "m", do: schannel_l InjL "m"),(λ: "m", do: schannel_l InjR "m"))%V) (f2 ((λ: "m", do: schannel_r InjL "m"),(λ: "m", do: schannel_r InjR "m"))%V) _ _ X' _ _ R _ _ _) with "[Hrelf1f2]"); simpl; first (set_solver); try done.
+ 
+   { About brel_introduction_mono.
+     set clt := ([channel'; getKey'; schannel_l], [leaksec'; schannel_r], X').
+     set cltheory := iLblSig_to_iLblThy [([channel'; getKey'; schannel_l] , [leaksec'; schannel_r] , X')].
+     set (L' := cltheory ++ (iLblSig_to_iLblThy L)).
+     set (keytheory := iLblSig_to_iLblThy [([keyleak1], [keyleak2], keyleak keyleak1 keyleak2)]).
+     set (leaktheory := (iLblSig_to_iLblThy [([leakauth1], [leakauth2], leakauth leakauth1 leakauth2)])).
+     set (M := cltheory ++ keytheory ++ leaktheory ++ (iLblSig_to_iLblThy L)).
+     About brel_introduction_mono.
+    iApply (brel_introduction_mono L' M).
+     + simpl.
+       Search to_iThy_le.
+       iApply to_iThy_le_intro'.
+       unfold L'. unfold M.  
+       Search " ⊆+". 
+       Search "++".
+       set (l := cltheory ++ keytheory ++ leaktheory).
+      
+       apply (submseteq_skips_r (iLblSig_to_iLblThy L) (cltheory) (cltheory ++ keytheory ++ leaktheory)).
+       eapply submseteq_inserts_r. eapply Permutation_submseteq. auto.
+     + unfold L'. iApply "Hrelf1f2". }
+   iLöb as "IH". 
+   iSplit; [iIntros (v1 v2) "%Hv1v2"; iModIntro; brel_pures; iModIntro; done |]. 
+   iIntros (?????) "!# %Hk1 %Hk2 HXQ #Hrel". 
+   iDestruct "HXQ" as "[HSendAlice | HRecvBob]".
+   (* Send to Bob*) 
+      + iDestruct "HSendAlice" as (?m ?m') "[[%He1 %He2] #HmQ]".         
+         rewrite -> He1. rewrite -> He2. brel_pures.
+         {  apply -> NeutralEctx_ectx_labels_singleton.
+           do 2 (eapply NeutralEctx_label_cons_inv_2 in Hk1). eapply Hk1. }
+         {  apply -> NeutralEctx_ectx_labels_singleton.
+            eapply NeutralEctx_label_cons_inv_2 in Hk2.
+            eapply NeutralEctx_label_cons_inv_1 in Hk2. eapply Hk2. } 
+         iApply (brel_na_inv _ _ betaN); first set_solver.
+         iFrame "Hinvβ".
+         iIntros "([(>Hl_fchan  & >Hl_rchan) | (#>Hl_fchan & #>Hl_rchan)] & Hclose)".
+         (* First message to be sent by the secure channel*)
+        ++  iApply (brel_load_r _ _ _ _ [HandleCtx _ _ _ _ _ ; CaseCtx _ _] with "Hl_fchan").
+             iIntros "Hl_fchan".
+             iApply (brel_load_l _ _ _  [HandleCtx Deep MS _ _ _ ; HandleCtx Deep MS _ _ _; CaseCtx _ _] with "Hl_rchan").
+             iIntros "!>Hl_rchan". brel_pures.
+             simpl. brel_pures. 
+             iApply (brel_store_r _ _ _ _ [HandleCtx _ _ _ _ _ ; AppRCtx _] with "Hl_fchan"). iIntros "Hl_fchan".
+             simpl.
+             brel_pures.
+             { simpl. apply not_elem_of_nil. }
+             iApply (brel_store_l _ _ _  [HandleCtx _ _ _ _ _ ; HandleCtx _ _ _ _ _ ; AppRCtx _] with "Hl_rchan").
+             iIntros "!>Hl_rchan". brel_pures; try (simpl); try (apply not_elem_of_nil).
+             iApply fupd_brel.
+             iMod (ghost_map_elem_persist with "Hl_fchan") as "#Hl_fchan".
+             iMod (ghost_map_elem_persist with "Hl_rchan") as "#Hl_rchan".
+             iModIntro.
+             iApply brel_na_close. iFrame.
+             iSplitL; [iModIntro; iRight; iFrame "#"|].
+            (* set (keytheory := [([keyleak1], [keyleak2],
+         iThySum (iThySum KLeakSendAlice KLeakRecvAlice)
+           (iThySum KLeakSendBob KLeakRecvBob))]).*)
+             (*set (keytheory := [([keyleak1], [keyleak2], keyleak keyleak1 keyleak2)]).*)
+            (*set (M := (([channel'; getKey'; schannel_l], [leaksec'; schannel_r], iThyBot)
+        :: ([leakauth1], [leakauth2], leakauth leakauth1 leakauth2) :: (iLblSig_to_iLblThy L))).
+            set (N := (([channel; getKey1; schannel1], [leaksec; schannel2; getKey2], iThyBot)
+     :: ([keyleak1], [keyleak2],
+         iThySum (iThySum KLeakSendAlice KLeakRecvAlice)
+           (iThySum KLeakSendBob KLeakRecvBob))
+        :: ([leakauth1], [leakauth2],
+             iThySum (iThySum LASendAlice LASendBob) (iThySum LARecvAlice LARecvBob)) :: L)).*)
+            simpl.
+            repeat foldkont.
+            simpl.
+            set (kontleftbind :=
+             (let: "r" := (λ: "m", do: keyleak1 "m")%V (InjR bob) in
+             match: "r" with
+               InjL <> => kont (InjLV #()%V)
+             | InjR "w" => kont (InjR (vgval (g ^+ n)))
+             end)%E).
+            set (kontrightbind := (let: "r" := (λ: "m", do: keyleak2 "m")%V (InjR bob) in
+     match: "r" with
+       InjL <> => kont0 (InjLV #()%V)
+     | InjR "x" =>
+       match: ! #l_sim with
+         InjL <> =>
+           let: "m'" := #()%V;; rand(#lbl:α) #(S n'') in
+           let: "mA" := vexp g "m'" in
+           #l_sim <- InjR "m'";; 
+           (λ: "m", do: leakauth2 Send "m")%V (InjL ("mA", bob));; kont0 #()%V
+       | InjR "m" => kont0 #()%V
+       end
+     end)%E).
+            About brel_bind''.
+            set (keytheory := iLblSig_to_iLblThy [([keyleak1], [keyleak2], keyleak keyleak1 keyleak2)]).
+            set (leaktheory := (iLblSig_to_iLblThy [([leakauth1], [leakauth2], leakauth leakauth1 leakauth2)])).
+            About leaktheory.
+            (*set (M := [([channel'; getKey'; schannel_l], [leaksec'; schannel_r], iThyBot Σ)]).*)
+            About brel_bind''.
+            set (M := [([channel'; getKey'; schannel_l], [leaksec'; schannel_r], @iThyBot Σ)] ++ leaktheory ++ (iLblSig_to_iLblThy L)).
+            set (N := [([channel'; getKey'; schannel_l], [leaksec'; schannel_r], @iThyBot Σ)] ++ keytheory ++ leaktheory ++ (iLblSig_to_iLblThy L)).
+           (* iApply (brel_bind'' [HandleCtx Deep _ _ _ _; AppRCtx _] [AppRCtx _] keytheory [([channel'; getKey'; schannel_l], [leaksec'; schannel_r], iThyBot)] (([leakauth1], [leakauth2], leakauth leakauth1 leakauth2) :: iLblSig_to_iLblThy L)  (λ v1 v2 : val, ⌜v1 = v2⌝%I) (Do keyleak1 (InjLV bob)) (Do keyleak2 (InjLV bob))).*)
+            iApply (brel_bind'' [HandleCtx Deep _ _ _ _; AppRCtx _] [AppRCtx _] keytheory M N (𝟙%T) (Do keyleak1 (InjLV bob)) (Do keyleak2 (InjLV bob))).
+             { simpl. unfold M. repeat (rewrite -> labels_l_cons). set_solver. }
+             { simpl. apply list_subseteq_nil. }
+             { simpl. unfold M. unfold N. iApply to_iThy_le_intro'. eapply Permutation_submseteq.
+               eapply perm_swap. } 
+             { iApply (brel_introduction' [keyleak1] [keyleak2]).
+                1: { unfold keytheory.
+                     eapply list_elem_of_here. }
+                iExists _, _, [], [],_.
+                do 2 (iSplit; [done|]; iSplit; [iPureIntro; apply _|]).
+                iSplitL;  [|by iIntros "!>" (??) "H"; iApply "H"].
+                iRight. iLeft. simpl. 
+                repeat (iSplit; try (iPureIntro); try (unfold SendV); try reflexivity).
+                iModIntro.
+                iApply brel_value.
+                iIntros "$ !>". brel_pures.
+                (*About brel_learn.*)
+                About distinct'. 
+                (*iAssert (distinct' (LblClients ++ L)) as "%Hdistinct".*)
+                iAssert (distinct' N) as "%Hdistinct".
+                { unfold N. unfold keytheory. unfold leaktheory. simpl.
+                  Print distinct.
+                  Print distinct'. unfold distinct'. iPureIntro. apply Hdist'. }
+                iApply (brel_bind'' _ _ keytheory M N 𝟙%T (Do keyleak1 (InjRV bob)) (Do keyleak2 (InjRV bob))).
+                { simpl. unfold M.  repeat (rewrite -> labels_l_cons). set_solver. }
+                { simpl. apply list_subseteq_nil. }
+                { simpl. unfold M. unfold N. iApply to_iThy_le_intro'. eapply Permutation_submseteq.
+               eapply perm_swap. }
+                { iApply (brel_introduction' [keyleak1] [keyleak2]).
+                1: { unfold keytheory.
+                     eapply list_elem_of_here. }
+                iExists _, _, [], [],_.
+                do 2 (iSplit; [done|]; iSplit; [iPureIntro; apply _|]).
+                iSplitL;  [|by iIntros "!>" (??) "H"; iApply "H"].
+                iRight. iRight. simpl.
+                repeat (iSplit; try (iPureIntro); try (unfold RecvV); try reflexivity);
+                  try (iModIntro); simpl.                                                                  iSplitL.
+                  +++ iApply brel_value.
+                      iIntros "$ !>". brel_pures.
+                      simpl. brel_pures.
+                      iApply (brel_exhaustion (fill k1' #()%V) (fill k2' #()%V)). 
+                      { simpl. auto. }
+                      { simpl. repeat (eapply list_subseteq_skip). eapply list_subseteq_nil. }
+                      { iApply "Hrel". iApply "HmQ". }
+                      { iApply "IH". }
+                  +++ iApply brel_value.
+                      iIntros "$ !>". brel_pures.
+                      { simpl. unfold distinct in Hdistinct. destruct Hdistinct.
+                        unfold distinct_l in H1. (*unfold LblClients in H1. simpl in H1.*)
+                        unfold N in H1. simpl in H1.
+                        repeat (rewrite -> labels_l_cons in H1).
+                        eapply NoDup_app in H1.
+                        eapply NoDup_cons_1_1. destruct H1 as [H1' H2'].
+                        apply (NoDup_app [channel'; getKey'] [schannel_l]) in H1'.
+                        destruct H1' as [H1' H2'']. apply H1'. }
+                      { simpl.
+                        iApply (brel_na_inv _ _ alphaN); first set_solver.
+                        iFrame "Hinvα".
+                        iIntros "([ (>Hα & >Hl_sim & >Hl_auth) | (#>Hα & #>Hl_sim & #>Hl_auth) ] & Hclose)". 
+                        (*first message to be sent by the authenticated channel*)
+                        - 
+                          iApply (brel_load_l _ _ _ [CaseCtx _ _] with "Hl_auth"). 
+                          (*iIntros "HvN HdN".
+                          iApply (rel_load_l_mask [CaseCtx _ _]).*)                                          
+                          iIntros "!> Hl_auth".
+                          simpl. brel_pures_l.
+                          (*iApply (rel_load_r_with_mask _ _ _ _ [CaseCtx _ _] with "Hl_sim").*) 
+                          iApply (brel_load_r _ _ _ _ [CaseCtx _ _] with "Hl_sim").
+                          iIntros "Hl_sim". rel_pures.
+                          iApply (brel_store_l _ _ _ [AppRCtx _] with "Hl_auth").
+                          iIntros "!> Hl_auth". brel_pures.
+                          iApply (brel_randT_r _ [AppRCtx _ ] with "Hα").
+                          iIntros "Hα %Hn".
+                          brel_pures.
+                          repeat foldkont.
+                          iApply (brel_exp_r [AppRCtx _]).
+                          brel_pures.
+                          iApply (brel_store_r _ _ _ _ [AppRCtx _] with "Hl_sim").
+                          iIntros "Hl_sim". rel_pures.
+                          iApply fupd_brel.
+                          iMod (ghost_map_elem_persist with "Hl_sim") as "#Hl_sim".
+                          iMod (ghost_map_elem_persist with "Hl_auth") as "#Hl_auth".
+                          (*iMod (ghost_map_elem_persist with "H") as "#Hl_fchan".*)
+                          iDestruct "Hα" as (ns) "(%Hf & Hα)".
+                          apply map_eq_nil in Hf. simplify_eq.
+                          iMod (ghost_map_elem_persist with "Hα") as "#Hα".
+                          iModIntro.
+                          iApply brel_na_close. iFrame.
+                          iSplitL; [iModIntro; iRight; iFrame "#"|].
+                          simpl.
+                          brel_pures. 
+                         (* set (leakatheory := [([leakauth1], [leakauth2],
+           iThySum (iThySum LASendAlice LASendBob)
+             (iThySum LARecvAlice LARecvBob))]).*)
+                          iApply (brel_bind _ _ _ leaktheory N _ (Do leakauth1 (InjLV (xor "x" "m", bob))) (Do leakauth2 (InjLV (vgval (g ^+ n) , bob)))).
+                          { simpl. unfold leaktheory. auto.
+                            Search "traversable".
+                            About traversable_ectx_labels.
+                            iApply (traversable_ectx_labels _ _ [] [] iThyBot _).
+                            + unfold kont1. simpl. auto.
+                            + unfold kont0. simpl. auto.
+                            + simpl. unfold distinct.
+                              unfold distinct_l, distinct_r.
+                              unfold labels_l, labels_r. simpl.
+                              Search "NoDup".
+                              split; eapply NoDup_singleton.
+                            }
+                            { simpl. unfold N. iApply to_iThy_le_intro'. 
+                              Search " ⊆+".
+                              set (k1 :=  [([channel'; getKey'; schannel_l], [leaksec'; schannel_r], iThyBot)] ++ keytheory).
+                              apply (submseteq_middle leaktheory k1 (iLblSig_to_iLblThy L)). }
+                          { iApply (brel_introduction' [leakauth1] [leakauth2]); try (unfold leaktheory);
+                            try (apply list_elem_of_here).
+                           iExists _, _, [], [],_.
+                do 2 (iSplit; [done|]; iSplit; [iPureIntro; apply _|]).
+                iSplitL;  [|by iIntros "!>" (??) "H"; iApply "H"].
+                iLeft. iLeft. simpl.
+                iExists _,_. repeat (iSplit; try (iPureIntro); try (unfold SendV); try reflexivity). 
+                iModIntro. iApply brel_value. iIntros "$ !>".
+                brel_pures. 
+                iApply (brel_exhaustion (fill k1' #()%V) (fill k2' #()%V)).
+                            { simpl. auto. }
+                            { simpl. auto. (*admit.*) }
+                            { iApply "Hrel". iApply "HmQ". }
+                            { iApply "IH". }          }                                                   
+                      (*a message has already been sent by the authenticated channel*)
+                        -  iApply brel_na_close. iFrame.
+                           iSplitL; [iModIntro; iRight; iFrame "#"|].
+                            iApply (brel_load_l _ _ _  [CaseCtx _ _] with "Hl_auth").
+                            iIntros "!> Hl_auth'".
+                            brel_pures.
+                            iApply (brel_load_r _ _ _ _  [CaseCtx _ _] with "Hl_sim").
+                            iIntros "Hl_sim'".
+                            brel_pures.
+                            iApply (brel_exhaustion (fill k1' #()%V) (fill k2' #()%V)).
+                            { simpl. auto. }
+                            { simpl. auto. (*admit.*) }
+                            { iApply "Hrel". iApply "HmQ". }
+                            { iApply "IH". } } } }
+         (* A message has already been sent by the secure channel*)
+        ++ iApply brel_na_close. iFrame.
+           iSplitL; [iModIntro; iRight; iFrame "#"|].
+           iApply (brel_load_l _ _ _  [HandleCtx _ _ _ _ _ ; HandleCtx _ _ _ _ _ ; CaseCtx _ _] with "Hl_rchan").
+           iIntros "!> Hl_rchan'".
+           brel_pures.
+           iApply (brel_load_r _ _ _ _  [HandleCtx _ _ _ _ _ ; CaseCtx _ _] with "Hl_fchan").
+           iIntros "Hl_fchan'".
+           brel_pures.
+           iApply (brel_exhaustion (fill k1' #()%V) (fill k2' #()%V)).
+           { simpl. auto. }
+           { simpl. auto. (*admit.*) }
+           { iApply "Hrel". iApply "HmQ". }
+           { iApply "IH". }
+     (* Recieved by Bob *)
+      + iDestruct "HRecvBob" as "[%He1 [%He2 #HmQ]]". 
+        rewrite -> He1. rewrite -> He2. brel_pures. 
+        { simpl. split; [| eapply not_elem_of_nil]. apply -> NeutralEctx_ectx_labels_singleton.
+           do 2 (eapply NeutralEctx_label_cons_inv_2 in Hk1). eapply Hk1. }
+        { simpl. split; [| eapply not_elem_of_nil]. apply -> NeutralEctx_ectx_labels_singleton.
+           eapply NeutralEctx_label_cons_inv_2 in Hk2. eapply Hk2. }
+         set (keytheory := iLblSig_to_iLblThy [([keyleak1], [keyleak2], keyleak keyleak1 keyleak2)]).
+         set (leaktheory := (iLblSig_to_iLblThy [([leakauth1], [leakauth2], leakauth leakauth1 leakauth2)])).
+         set (M := [([channel'; getKey'; schannel_l], [leaksec'; schannel_r], @iThyBot Σ)]).
+         (* ++ leaktheory ++ (iLblSig_to_iLblThy L)) *)
+         set (N := [([channel'; getKey'; schannel_l], [leaksec'; schannel_r], @iThyBot Σ)] ++ keytheory ++ leaktheory ++ (iLblSig_to_iLblThy L)).
+       (* set (N := (([channel; getKey1; schannel1], [leaksec; schannel2; getKey2],
+      iThyBot)
+     :: ([keyleak1], [keyleak2],
+         iThySum (iThySum KLeakSendAlice KLeakRecvAlice)
+           (iThySum KLeakSendBob KLeakRecvBob))
+        :: ([leakauth1], [leakauth2],
+            iThySum (iThySum LASendAlice LASendBob)
+              (iThySum LARecvAlice LARecvBob))
+        :: L)).
+        set (keyleakthy := [([keyleak1], [keyleak2],
+         iThySum (iThySum KLeakSendAlice KLeakRecvAlice)
+           (iThySum KLeakSendBob KLeakRecvBob))]).
+        set (M := [([channel; getKey1; schannel1],
+                 [leaksec; schannel2; getKey2], SecChannelThy)]).*)
+        iApply (brel_bind'' _ _ keytheory M N _ (Do keyleak1 (InjLV bob)) (Do keyleak2 (InjLV bob))).
+        { simpl. unfold M. unfold labels_l. simpl. Search "⊆".  apply (list_subseteq_skip channel' [] [getKey'; schannel_l]). set_solver. }
+        { simpl. unfold M. unfold labels_r. simpl. set_solver. }
+        { iApply to_iThy_le_intro'. unfold M. unfold N. Search "⊆+".
+          eapply submseteq_sublist_r.
+          exists ([([channel'; getKey'; schannel_l], [leaksec'; schannel_r],
+                 iThyBot)] ++ keytheory). split.
+          + repeat simpl. unfold keytheory. simpl. eapply Permutation_swap.
+          + Search "`sublist_of`".
+            set (l1 :=  [([channel'; getKey'; schannel_l], [leaksec'; schannel_r],
+                            iThyBot)] ++ keytheory).
+            set (l2 := leaktheory ++ iLblSig_to_iLblThy L).
+            Print sublist_inserts_r.
+            apply (sublist_inserts_r l2 l1 l1). auto. }
+        {  iApply (brel_introduction' [keyleak1] [keyleak2]).
+                1: { unfold keytheory.
+                     eapply list_elem_of_here. }
+                iExists _, _, [], [],_.
+                do 2 (iSplit; [done|]; iSplit; [iPureIntro; apply _|]).
+                iSplitL;  [|by iIntros "!>" (??) "H"; iApply "H"].
+                iRight. iLeft. simpl.
+                repeat (iSplit; try (iPureIntro); try (unfold SendV); try reflexivity).
+                iModIntro. iApply brel_value. 
+                iIntros "$ !>". brel_pures.
+                iApply (brel_bind'' _ _ keytheory M N _ (Do keyleak1 (InjRV bob)) (Do keyleak2 (InjRV bob))).
+                { simpl. unfold M. unfold labels_l. simpl. Search "⊆".  apply (list_subseteq_skip channel' [] [getKey'; schannel_l]). set_solver. }
+                { simpl. unfold M. unfold labels_r. simpl. set_solver. }
+                {  iApply to_iThy_le_intro'. unfold M. unfold N. Search "⊆+".
+          eapply submseteq_sublist_r.
+          exists ([([channel'; getKey'; schannel_l], [leaksec'; schannel_r],
+                 iThyBot)] ++ keytheory). split.
+          + repeat simpl. unfold keytheory. simpl. eapply Permutation_swap.
+          + Search "`sublist_of`".
+            set (l1 :=  [([channel'; getKey'; schannel_l], [leaksec'; schannel_r],
+                            iThyBot)] ++ keytheory).
+            set (l2 := leaktheory ++ iLblSig_to_iLblThy L).
+            Print sublist_inserts_r.
+            apply (sublist_inserts_r l2 l1 l1). auto. }
+                {  iApply (brel_introduction' [keyleak1] [keyleak2]).
+                1: { unfold keytheory.
+                     eapply list_elem_of_here. }
+                iExists _, _, [], [],_.
+                do 2 (iSplit; [done|]; iSplit; [iPureIntro; apply _|]).
+                iSplitL;  [|by iIntros "!>" (??) "H"; iApply "H"].
+                iRight. iRight. simpl.
+                repeat (iSplit; try (iPureIntro); try (unfold RecvV); try reflexivity).
+                iModIntro. iSplitL; iApply brel_value; iIntros "$ !>" ; brel_pures.
+                (* Key not received by Bob*)
+                   ++ iApply (brel_exhaustion (fill k1'(InjLV #()%V)) (fill k2' (InjLV #()%V))). 
+                      { simpl. auto. }
+                      { simpl. auto. (*admit.*) }
+                      { iApply "Hrel". iDestruct "HmQ" as "[Hsome Hnone]". iApply "Hnone". }
+                      { iApply "IH". }
+                      (* Key received by Bob *)
+                   ++  simpl. unfold distinct in Hdist'. destruct Hdist' as [Hdl HdR].
+                       unfold distinct_l in Hdl. unfold labels_l in Hdl. simpl in Hdl.
+                       Search "NoDup".
+                       assert (HNoDup : NoDup [channel'; getKey']).
+                       { About sublist_NoDup. eapply sublist_NoDup; [eapply Hdl| auto].
+                         eapply (sublist_inserts_r _ [channel'; getKey'] [channel'; getKey']). auto. }
+                       Search "NoDup". apply NoDup_cons_1_1 in HNoDup. auto.
+                   ++ (*set (leakauththy := [([leakauth1], [leakauth2],
+                       iThySum (iThySum LASendAlice LASendBob) (iThySum LARecvAlice LARecvBob))]).*) 
+                      iApply (brel_bind'' _ _ leaktheory M N _ (Do leakauth1 (InjRV bob)) (Do leakauth2 (InjRV bob))).
+                      { simpl. unfold M. unfold labels_l. simpl. set_solver. }
+                      { simpl. unfold M. unfold labels_r. simpl. set_solver. }
+                      {  iApply to_iThy_le_intro'. unfold M. unfold N. Search "⊆+".
+          eapply submseteq_sublist_r.
+          exists ([([channel'; getKey'; schannel_l], [leaksec'; schannel_r],
+                 iThyBot)] ++ leaktheory). split.
+          + repeat simpl. unfold leaktheory. simpl. eapply Permutation_swap.
+          + Search "`sublist_of`".
+            eapply sublist_skip. eapply sublist_inserts_l. eapply sublist_inserts_r. auto. }
+                      { iApply (brel_introduction' [leakauth1] [leakauth2]).
+                        1: { unfold leaktheory.
+                             eapply list_elem_of_here. }
+                        simpl.
+                        iExists _, _, [], [],_.
+                        do 2 (iSplit; [done|]; iSplit; [iPureIntro; apply _|]).
+                        iSplitL;  [|by iIntros "!>" (??) "H"; iApply "H"].
+                        iRight. iRight. simpl.
+                        repeat (iSplit; try (iPureIntro); try (unfold RecvV); try reflexivity).
+                        iModIntro. iSplit.
+                        (* leakauth returns successfully with a value*)
+                        - iIntros (b1 b2). iApply brel_value. iIntros "$ !>".
+                          brel_pures. simpl.
+                          iApply (brel_na_inv _ _ alphaN); first set_solver.
+                          iFrame "Hinvα".
+                          iIntros "([ (>Hα & >Hl_sim & >Hl_auth) | (#>Hα & #>Hl_sim & #>Hl_auth) ] & Hclose)".
+                          (* first case, when no message is stored in the authenticated channel*)
+                          +++ simpl. brel_pures.
+                              iApply (brel_load_r _ _ _ _ [AppRCtx _] with "Hl_sim").
+                              iIntros "Hl_sim".
+                              iApply (brel_load_l _ _ _ [AppRCtx _] with "Hl_auth").
+                              iIntros "!>Hl_auth".
+                              simpl.
+                              brel_pures.
+                              iApply brel_na_close. iFrame.
+                              iSplitL; [iModIntro; iLeft; iFrame |].
+                              iApply (brel_exhaustion (fill k1'(InjLV #()%V)) (fill k2' (InjLV #()%V))).
+                               { simpl. auto. }
+                               { simpl. set_solver. }
+                               { iApply "Hrel". iDestruct "HmQ" as "[Hsome Hnone]". iApply "Hnone". }
+                               { iApply "IH". }
+                               (*second case for the invariant, when a message is stored in the authenticated channel*)
+                          +++ simpl. brel_pures.
+                              iApply (brel_load_r _ _ _ _ [AppRCtx _] with "Hl_sim").
+                              iIntros "Hl_sim'".
+                              iApply (brel_load_l _ _ _ [AppRCtx _] with "Hl_auth").
+                              iIntros "!>Hl_auth'".
+                              simpl.
+                              brel_pures.
+                              iApply brel_na_close. iFrame.
+                              iSplitL; [iModIntro; iRight; iFrame "#" |].
+                              iApply (brel_exhaustion (fill k1'((InjRV (xor "key" "x"))%V)) (fill k2' ((InjRV #n)%V))).
+                               { simpl. auto. }
+                               { simpl. set_solver. }
+                               { iApply "Hrel". iDestruct "HmQ" as "[Hsome Hnone]". unfold xor. iApply "Hsome". }
+                               { iApply "IH". } 
+                         (*leakauth doesnot return with a value*)                             
+                        - brel_pures.
+                          iApply brel_value.
+                          iIntros "$ !>". brel_pures.
+                          iApply (brel_exhaustion (fill k1' (InjLV #()%V)) (fill k2' (InjLV #()%V))).
+                          { simpl. auto. }
+                          { simpl. set_solver. }
+                          { iApply "Hrel".  iDestruct "HmQ" as "[Hsome Hnone]". unfold xor. iApply "Hnone". }
+                          {iApply "IH". } } } }
+                          
+Qed.
  
 End schan_security.
